backend/Mach.v
@@ -446,7 +446,8 @@ Inductive step: state -> trace -> state -> Prop :=
       forall (CALLED: Genv.find_funct_ptr ge f' = Some fd),
       forall (ALLOWED: comp_of fd = comp_of f),
       forall (SIG: sig = funsig fd),
-      forall (ARGS: call_arguments (undef_regs destroyed_at_function_entry rs) m sp sig args), (* simpler for later pass*)
+      forall (ARGS: call_arguments
+                 (undef_regs destroyed_at_function_entry rs) m sp sig args), (* simpler for later pass*)
       step (State s fb sp (Mcall sig ros :: c) rs m)
         E0 (Callstate (Stackframe fb sig sp ra c None None :: s)
                        f' sig rs m (comp_of f))
